cbor_serialize_array

src/cbor/pulse/raw/CBOR.Pulse.Raw.Format.Serialize.fsti
@@ -5,6 +5,7 @@ open Pulse.Lib.Pervasives
 open Pulse.Lib.Trade
 
 module U8 = FStar.UInt8
+module U64 = FStar.UInt64
 module SZ = FStar.SizeT
 module Trade = Pulse.Lib.Trade.Util
 module S = Pulse.Lib.Slice
@@ -63,3 +64,38 @@ val cbor_serialize_tag
 : stt SZ.t
   (exists* v . pts_to output v)
   (fun res -> exists* v . pts_to output v ** pure (cbor_serialize_tag_postcond tag output res v))
+
+let cbor_serialize_array_precond
+  (len: raw_uint64)
+  (l: list raw_data_item)
+  (off: SZ.t)
+  (v: Seq.seq U8.t)
+: Tot prop
+= SZ.v off <= Seq.length v /\
+  Seq.slice v 0 (SZ.v off) == serialize_cbor_list l /\
+  List.Tot.length l == U64.v len.value
+
+let cbor_serialize_array_postcond
+  (len: raw_uint64)
+  (l: list raw_data_item)
+  (res: SZ.t)
+  (v: Seq.seq U8.t)
+: Tot prop
+= List.Tot.length l == U64.v len.value /\
+  SZ.v res <= Seq.length v /\
+  (res == 0sz <==> Seq.length (serialize_cbor (Array len l)) > Seq.length v) /\
+  (SZ.v res > 0 ==> Seq.slice v 0 (SZ.v res) `Seq.equal` serialize_cbor (Array len l))
+
+val cbor_serialize_array
+  (len: raw_uint64)
+  (out: S.slice U8.t)
+  (l: Ghost.erased (list raw_data_item))
+  (off: SZ.t)
+: stt SZ.t
+  (exists* v . pts_to out v **
+    pure (cbor_serialize_array_precond len l off v)
+  )
+  (fun res -> exists* v .
+    pts_to out v **
+    pure (cbor_serialize_array_postcond len l res v)
+  )
